theories/examples/local.v
@@ -1,134 +1,93 @@
-From iris.proofmode Require Import coq_tactics reduction spec_patterns.
-From iris.proofmode Require Export tactics.
-From iris.prelude Require Import options.
-From melocoton Require Import named_props.
-From melocoton.ml_lang.logrel Require logrel typing fundamental.
-From melocoton.interop Require Import basics basics_resources.
-From melocoton.lang_to_mlang Require Import lang weakestpre.
-From melocoton.interop Require Import lang weakestpre update_laws wp_utils wp_ext_call_laws wp_simulation.
-From melocoton.c_interop Require Import rules.
-From melocoton.ml_lang Require Import notation lang_instantiation.
-From melocoton.c_lang Require Import mlang_instantiation lang_instantiation.
-From melocoton.ml_lang Require proofmode.
-From melocoton.c_lang Require notation proofmode.
-From melocoton.mlanguage Require Import progenv.
-From melocoton.mlanguage Require weakestpre.
-From melocoton.linking Require Import lang weakestpre.
-From melocoton.combined Require Import adequacy rules.
+From iris.proofmode   Require Import coq_tactics reduction spec_patterns.
+From iris.proofmode   Require Export tactics.
+From iris.prelude     Require Import options.
+From melocoton        Require Import named_props.
+From melocoton.c_lang Require Import lang notation proofmode.
 
-Section FFI_spec.
+Context `{SI:indexT}.
+Context `{!heapG_C Σ, !invG Σ}.
 
-  Import melocoton.c_interop.notation melocoton.c_lang.proofmode.
+Tactic Notation "wp_allocframe" ident(fp) uconstr(Hfp) :=
+  wp_pures;
+  wp_apply (wp_allocframe);
+  iIntros (fp) "Hfp"; unfold allocate_frame; cbn -[array]; wp_pures.
 
-  Context `{SI:indexT}.
-  Context `{!ffiG Σ}.
+Section One.
 
-  Definition caml_incr : expr :=
-    "p" <- *"p" + #C 1;;
-    #C LitNull.
+  Definition addr : expr :=
+    &: "e".
+
+  Definition arg_prog : lang_prog C_lang :=
+    {[ "addr" := Fun [BNamed "e"] addr ]}.
+
+  Definition arg_prog_spec : protocol val Σ :=
+    !! e {{ True }} "addr" with [e] {{ (l : loc), RET(#C l); True }}.
+
+  Lemma arg_correct:
+    ||- arg_prog :: arg_prog_spec.
+  Proof.
+    iIntros (ψext x lvs ϕ) "H". iNamed "H". iSplit; first done.
+    iIntros (Φ') "HΦ". iNamed "H".
+
+    wp_allocframe fp "Hfp".
+    wp_apply (wp_free_array with "Hfp").
+    iIntros "_". wp_pures.
+    iModIntro. iApply "HΦ". by iApply "Cont".
+  Qed.
+
+End One.
+
+Section Two.
+
+  Definition id : expr :=
+    let: "_" := &: "e" in
+    "e".
+
+  Definition id_prog : lang_prog C_lang :=
+    {[ "id" := Fun [BNamed "e"] id ]}.
+
+  Definition id_spec : protocol val Σ :=
+    !! e {{ True }} "id" with [e] {{ RET(e); True }}.
+
+  Lemma id_correct:
+    ||- id_prog :: id_spec.
+  Proof.
+    iIntros (ψext x lvs ϕ) "H". iNamed "H". iSplit; first done.
+    iIntros (Φ') "HΦ". iNamed "H".
+    wp_call_direct.
+    wp_allocframe fp "Hfp".
+  Admitted.
+
+End Two.
+
+Section Three.
+
+  Definition incr : expr :=
+    "p" <- *"p" + #C 1.
 
   (* Times two plus one *)
-  Definition caml_ttpo : expr :=
+  Definition ttpo : expr :=
     let: "e2" := "e" in
-    call: "caml_incr" with (&: "e");;
+    call: &"incr" with (&: "e");;
     "e2" + "e".
 
-  Definition caml_local_prog : lang_prog C_lang :=
+  Definition ttpo_prog : lang_prog C_lang :=
     {[
-      "caml_incr" := Fun [BNamed "p"] caml_incr;
-      "caml_ttpo" := Fun [BNamed "e"] caml_ttpo
+      "incr" := Fun [BNamed "p"] incr;
+      "ttpo" := Fun [BNamed "e"] ttpo
     ]}.
 
-  Definition caml_local_spec : protocol ML_lang.val Σ :=
-    !! e (n : Z)
-      {{ ⌜e = #ML n⌝ }}
-        "caml_ttpo" with [e]
-      {{
-        RET((#ML (n + n + 1)) %MLV);
-        True
-      }}.
+  Definition ttpo_spec : protocol val Σ :=
+    !! e (n : Z) {{ ⌜e = #C n⌝ }} "ttpo" with [e] {{ RET(#C (n + n + 1)); True }}.
 
-  Lemma caml_local_correct:
-    prims_proto caml_local_spec
-    ||- caml_local_prog :: wrap_proto caml_local_spec.
+  Lemma ttpo_correct:
+    ||- ttpo_prog :: ttpo_spec.
   Proof.
-    iIntros (fn ws Φ) "H". iNamed "H". iNamedProto "Hproto".
-    iSplit; first done. iIntros (Φ'') "HΦ".
-    iAssert (⌜length lvs = 1⌝)%I as %Hlen.
-    { by iDestruct (big_sepL2_length with "Hsim") as %?. }
-    destruct lvs as [|lv []]; try by (exfalso; eauto with lia); []. clear Hlen.
-    destruct ws as [|w []]; try by (exfalso; apply Forall2_length in Hrepr; eauto with lia); [].
-    apply Forall2_cons_1 in Hrepr as [Hrepr _].
-    cbn.
-    iDestruct "Hsim" as "[He _ ]".
+    iIntros (ψext x lvs ϕ) "H". iNamed "H". iSplit; first done.
+    iIntros (Φ') "HΦ". iNamed "H".
     wp_call_direct.
+    wp_allocframe fp "Hfp".
+    wp_apply (wp_load).
+  Admitted.
 
-    wp_pures.
-    (* Allocate result variable *)
-    wp_apply (wp_alloc_foreign with "[$HGC]"); try eauto.
-    iIntros (θ' γ w) "(HGC&Hγ&%Hγw)". wp_pures.
-
-    (* Populate result variable *)
-    wp_apply (wp_write_foreign with "[$HGC $Hγ]"); try eauto.
-    iIntros "(HGC&Hγ)". wp_pures.
-
-    iMod (freeze_foreign_to_immut γ θ' _ with "[$]") as "(HGC&#Hγ)".
-
-    iModIntro.
-    iApply "HΦ".
-    iApply ("Return" with "[$HGC] [Cont] []").
-    - by iApply "Cont".
-    - cbn. iExists γ. iSplit; try eauto.
-    - eauto.
-Qed.
-
-End FFI_spec.
-
-Section ML_spec.
-  Import melocoton.ml_lang.proofmode.
-  Import logrel typing fundamental.
-
-  Context `{SI:indexT}.
-  Context `{!ffiG Σ}.
-  Context `{!logrelG Σ}.
-
-  Definition program_type_ctx : program_env :=
-    {[ "caml_new_boxedint" := FunType [] (TBoxedNat) ]}.
-
-  Lemma new_boxedint_well_typed Δ : ⊢ ⟦ program_type_ctx ⟧ₚ* ⟨∅, caml_new_boxedint_spec⟩ Δ.
-  Proof.
-    iIntros (s vv Φ) "!> (%ats&%rt&%Heq&Hargs&Htok&HCont)".
-    wp_extern. iModIntro. unfold program_type_ctx in Heq.
-    apply lookup_singleton_Some in Heq as (<-&Heq). simplify_eq.
-    iPoseProof (big_sepL2_length with "Hargs") as "%Heq".
-    destruct vv as [|v [|??]]; cbn in Heq; try lia.
-    cbn.
-    do 3 (iSplit; first done).
-    iIntros "!> _". wp_pures. iModIntro.
-    iApply ("HCont" with "[-Htok] Htok").
-    iExists 0. done.
-  Qed.
-
-End ML_spec.
-
-Section ML_Example.
-
-  Import melocoton.ml_lang.proofmode.
-
-  Context `{SI:indexT}.
-  Context `{!ffiG Σ}.
-
-  Definition new_boxedint_client : mlanguage.expr (lang_to_mlang ML_lang) :=
-    (Extern "caml_new_boxedint" []).
-
-  Lemma ML_prog_correct_axiomatic :
-    ⊢ WP new_boxedint_client at ⟨∅, caml_new_boxedint_spec⟩
-      {{ v, ⌜∃x : Z, v = OVal (#ML (LitBoxedInt x))⌝}}.
-  Proof.
-    unfold new_boxedint_client. wp_pures. wp_extern.
-    iModIntro. cbn.
-    do 3 (iSplitR; first done). iIntros "!> _".
-    wp_pures. iModIntro. iPureIntro. eauto.
-  Qed.
-
-End ML_Example.
+End Three.
